wip on switching to Z instead of nat and simplifying load/store_word_list
(committing wip from July 5th before continuing)

src/Memory.v
@@ -2,41 +2,45 @@ Require Import Coq.Lists.List.
 Require Import bbv.Word.
 Require Import Coq.omega.Omega.
 Require Import Coq.micromega.Lia.
-Require Import riscv.util.nat_div_mod_to_quot_rem.
+Require Import riscv.util.div_mod_to_quot_rem.
 Require Import riscv.util.Tactics.
 Require Import riscv.Utility.
+
+
+Local Open Scope Z_scope.
 
 Section ValidAddr.
 
 Context {t: Set}.
 Context {MW: MachineWidth t}.
 
-Definition valid_addr(addr: t)(alignment size: nat): Prop :=
-  regToNat addr + alignment <= size /\ (regToNat addr) mod alignment = 0.
+Definition valid_addr(addr: t)(alignment size: Z): Prop :=
+  regToZ_unsigned addr + alignment <= size /\ (regToZ_unsigned addr) mod alignment = 0.
 
 (* Note: alignment refers to addr, not to the range *)
-Definition in_range(addr: t)(alignment start size: nat): Prop :=
-  start <= regToNat addr /\
-  regToNat addr + alignment <= start + size /\
-  regToNat addr mod alignment = 0.
+Definition in_range(addr: t)(alignment start size: Z): Prop :=
+  start <= regToZ_unsigned addr /\
+  regToZ_unsigned addr + alignment <= start + size /\
+  regToZ_unsigned addr mod alignment = 0.
 
-Definition not_in_range(addr: t)(alignment start size: nat): Prop :=
-  regToNat addr + alignment <= start \/ start + size <= regToNat addr.
+Definition not_in_range(addr: t)(alignment start size: Z): Prop :=
+  regToZ_unsigned addr + alignment <= start \/ start + size <= regToZ_unsigned addr.
 
-Definition valid_addr'(addr: t)(alignment size: nat): Prop :=
+Definition valid_addr'(addr: t)(alignment size: Z): Prop :=
   in_range addr alignment 0 size.
 
 Lemma valid_addr_alt: forall (addr: t) alignment size,
     valid_addr addr alignment size <-> valid_addr' addr alignment size.
 Proof.
   intros. unfold valid_addr, valid_addr', in_range.
+  pose proof (regToZ_unsigned_bounds addr).
   intuition omega.
 Qed.
 
 End ValidAddr.
 
 Class Memory(m t: Set)`{MachineWidth t} := mkMemory {
-  memSize: m -> nat;
+  memSize: m -> Z;
 
   loadByte   : m -> t -> word  8;
   loadHalf   : m -> t -> word 16;
@@ -135,7 +139,7 @@ Lemma valid_addr_8_4: forall {t: Set} {MW: MachineWidth t} (addr: t) size,
 Proof.
   intros. unfold valid_addr in *.
   intuition (try omega).
-  nat_div_mod_to_quot_rem.
+  div_mod_to_quot_rem.
   nia.
 Qed.
 
@@ -144,9 +148,9 @@ Lemma list_elementwise_same: forall A (l1 l2: list A),
     l1 = l2.
 Proof.
   induction l1; intros.
-  - specialize (H 0). simpl in H. destruct l2; congruence.
+  - specialize (H O). simpl in H. destruct l2; congruence.
   - pose proof H as G.
-    specialize (H 0). simpl in H. destruct l2; inversion H. subst. f_equal.
+    specialize (H O). simpl in H. destruct l2; inversion H. subst. f_equal.
     apply IHl1. intro i. apply (G (S i)).
 Qed.
 
@@ -172,6 +176,82 @@ Proof.
   - destruct l; simpl in *; try discriminate. apply IHn. assumption.
 Qed.
 
+Definition map_nat_range{R: Type}(f: nat -> R): nat -> nat -> list R :=
+  fix rec(start count: nat) :=
+    match count with
+    | O => nil
+    | S count' => f start :: rec (S start) count'
+    end.
+
+Definition map_range{R: Type}(f: Z -> R)(count: Z): list R :=
+  map_nat_range (fun i => f (Z.of_nat i)) 0 (Z.to_nat count).
+
+Definition fold_left_index{A B: Type}(f: Z -> A -> B -> A)(l: list B)(i0: Z)(a0: A): A :=
+  snd (fold_left (fun p b => (fst p + 1, f (fst p) (snd p) b)) l (i0, a0)).
+
+Definition Znth_error{A: Type}(l: list A)(i: Z): option A :=
+  match i with
+  | Zneg _ => None
+  | _ => nth_error l (Z.to_nat i)
+  end.
+
+Definition Zlength{T: Type}(l: list T): Z := Z.of_nat (length l).
+
+Lemma length_map_nat_range{R: Type}: forall (f: nat -> R) (count start: nat),
+    length (map_nat_range f start count) = count.
+Proof.
+  induction count; intros; simpl; congruence.
+Qed.
+
+Lemma Zlength_map_range{R: Type}: forall (f: Z -> R) (count: Z),
+    0 <= count ->
+    Zlength (map_range f count) = count.
+Proof.
+  intros. unfold map_range, Zlength.
+  rewrite length_map_nat_range.
+  apply Z2Nat.id.
+  assumption.
+Qed.
+
+Lemma nth_error_map_nat_range{R: Type}: forall (f: nat -> R) (count start i: nat),
+    (start <= i < start + count)%nat ->
+    nth_error (map_nat_range f start count) (i - start) = Some (f i).
+Proof.
+  induction count; intros.
+  - exfalso. omega.
+  - simpl. assert (start = i \/ start < i)%nat as C by omega. destruct C as [C | C].
+    + subst. rewrite Nat.sub_diag. reflexivity.
+    + destruct i; [exfalso;omega|].
+      replace (S i - start)%nat with (S (i - start)) by omega.
+      simpl.
+      specialize (IHcount (S start) (S i)).
+      rewrite Nat.sub_succ in IHcount.
+      apply IHcount.
+      omega.
+Qed.
+
+Lemma Znth_error_map_range{R: Type}: forall (f: Z -> R) (count i: Z),
+    0 <= i < count ->
+    Znth_error (map_range f count) i = Some (f i).
+Proof.
+  intros. unfold Znth_error, map_range.
+  pose proof (@nth_error_map_nat_range R) as P.
+  specialize P with (start := O).
+  setoid_rewrite Nat.sub_0_r in P.
+  destruct i.
+  - rewrite P.
+    + reflexivity.
+    + split; [omega|].
+      apply Z2Nat.inj_lt; omega.
+  - rewrite P.
+    + f_equal. f_equal. apply Z2Nat.id. omega.
+    + split; [omega|].
+      rewrite Nat.add_0_l.
+      apply Z2Nat.inj_lt; omega.
+  - exfalso. destruct H as [H _].
+    unfold Z.le in H. simpl in H. congruence.
+Qed.    
+
 Ltac demod :=  
   repeat match goal with
          | H: _ mod _ = 0 |- _ => apply Nat.mod_divides in H; [destruct H | congruence]
@@ -179,7 +259,7 @@ Ltac demod :=
 
 (* destruct list length without destructing the cons to avoid unwanted simpls *)
 Lemma destruct_list_length: forall A (l: list A),
-    l = nil /\ length l = 0 \/ length l = S (pred (length l)).
+    l = nil /\ length l = O \/ length l = S (pred (length l)).
 Proof.
   intros. destruct l; simpl; auto.
 Qed.
@@ -191,44 +271,6 @@ Ltac destruct_list_length :=
        destruct (destruct_list_length _ L) as [ [ ? ? ] | ? ]; [ subst L | ]
   end.
 
-Local Arguments Nat.modulo: simpl never.
-
-Lemma mod_0_r: forall (m: nat),
-    m mod 0 = 0.
-Proof.
-  intros. reflexivity.
-Qed.
-
-Lemma sub_mod_0: forall (a b m: nat),
-    a mod m = 0 ->
-    b mod m = 0 ->
-    (a - b) mod m = 0.
-Proof.
-  intros. assert (m = 0 \/ m <> 0) as C by omega. destruct C as [C | C].
-  - subst. apply mod_0_r.
-  - assert (a - b = 0 \/ b < a) as D by omega. destruct D as [D | D].
-    + rewrite D. apply Nat.mod_0_l. assumption.
-    + apply Nat2Z.inj. simpl.
-      rewrite Zdiv.mod_Zmod by assumption.
-      rewrite Nat2Z.inj_sub by omega.
-      rewrite Zdiv.Zminus_mod.
-      rewrite <-! Zdiv.mod_Zmod by assumption.
-      rewrite H. rewrite H0.
-      apply Z.mod_0_l.
-      omega.
-Qed.      
-
-Lemma wminus_minus': forall (sz : nat) (a b : word sz),
-    #b <= #a ->
-    #(a ^- b) = #a - #b.
-Proof.
-  intros. apply wminus_minus.
-  unfold wlt. intro C.
-  apply Nlt_out in C.
-  rewrite! wordToN_to_nat in *.
-  omega.
-Qed.
-
 Ltac womega_pre :=
   match goal with
   | |- ~ (@eq (word _) _ _) => apply wordToNat_neq2
@@ -237,15 +279,7 @@ Ltac womega_pre :=
 
 Ltac womega := womega_pre; omega.
 
-Lemma mul_div_exact: forall (a b: nat),
-    b <> 0 ->
-    a mod b = 0 ->
-    b * (a / b) = a.
-Proof.
-  intros. edestruct Nat.div_exact as [_ P]; [eassumption|].
-  specialize (P H0). symmetry. exact P.
-Qed.
-
+(*
 Hint Rewrite
      Nat.succ_inj_wd
      Nat.mul_0_r
@@ -254,6 +288,7 @@ Hint Rewrite
      mul_div_exact
 using omega
 : nats.
+ *)
 
 Ltac pose_mem_proofs :=
   repeat match goal with
@@ -289,9 +324,29 @@ Section MemoryHelpers.
   Context {t: Set}.
   Context {MW: MachineWidth t}.
   Context {MM: Memory Mem t}.
-  Hypothesis pow2_sz_4: 4 < pow2 XLEN.
+  Hypothesis pow2_sz_4: 4 < 2 ^ XLEN.
 
   Add Ring tring: (@regRing t MW).
+
+  Lemma regToZ_unsigned_one: regToZ_unsigned one = 1.
+  Proof.
+    intros. rewrite <- ZToReg_morphism.(morph1).
+    apply regToZ_ZToReg_unsigned. omega.
+  Qed.
+
+  Lemma regToZ_unsigned_two: regToZ_unsigned two = 2.
+  Proof.
+    intros. unfold two. rewrite add_def_unsigned.
+    rewrite regToZ_unsigned_one.
+    apply regToZ_ZToReg_unsigned. omega.
+  Qed.
+  
+  Lemma regToZ_unsigned_four: regToZ_unsigned four = 4.
+  Proof.
+    intros. unfold four. rewrite add_def_unsigned.
+    rewrite regToZ_unsigned_two.
+    apply regToZ_ZToReg_unsigned. omega.
+  Qed.
 
   Lemma loadWord_storeDouble_ne: forall m (a1 a2: t) v,
       valid_addr a1 8 (memSize m) ->
@@ -304,22 +359,23 @@ Section MemoryHelpers.
     pose proof (memSize_bound m) as B.
     pose proof loadStoreDouble_ne as P.
     specialize P with (1 := H).
-    destruct (mod2_cases (regToNat a2 / 4)) as [C | C].
+    Search (_ mod 2)%Z.
+    destruct (ZLib.mod2_cases (regToZ_unsigned a2 / 4)) as [C | C].
     - specialize (P a2 v).
       assert (valid_addr a2 8 (memSize m)) as V. {
         unfold valid_addr in *.
         destruct H, H0.
-        assert (regToNat a2 mod 8 = 0). {
-          apply Nat.mod_divide; try congruence.
+        assert (regToZ_unsigned a2 mod 8 = 0). {
+          apply Z.mod_divide; try congruence.
           change 8 with (2 * 4).
-          replace (regToNat a2) with (regToNat a2 / 4 * 4).
-          - apply Nat.mul_divide_mono_r.
-            apply Nat.mod_divide; try congruence.
-          - apply div_mul_undo; congruence.
+          replace (regToZ_unsigned a2) with (regToZ_unsigned a2 / 4 * 4).
+          - apply Z.mul_divide_mono_r.
+            apply Z.mod_divide; congruence.
+          - apply ZLib.div_mul_undo; congruence.
         }
         split; try assumption.
         pose proof (memSize_mod8 m).
-        demod. omega.
+        div_mod_to_quot_rem. omega.
       }
       specialize (P V).
       rewrite loadDouble_spec in P
@@ -327,10 +383,15 @@ Section MemoryHelpers.
       specialize (P H1).
       rewrite loadDouble_spec in P by assumption.
       pose proof combine_inj as Q.
-      specialize (Q 32 32 _ _ _ _ P).
+      specialize (Q 32%nat 32%nat _ _ _ _ P).
       destruct Q as [Q _]. assumption.
     - specialize (P (sub a2 four) v).
-      assert (regToNat a2 = 0 \/ regToNat a2 = 1 \/ regToNat a2 = 2 \/ regToNat a2 = 3 \/ 4 <= regToNat a2) as D by omega.
+      pose proof (regToZ_unsigned_bounds a2).
+      assert (regToZ_unsigned a2 = 0 \/
+              regToZ_unsigned a2 = 1 \/
+              regToZ_unsigned a2 = 2 \/
+              regToZ_unsigned a2 = 3 \/
+              4 <= regToZ_unsigned a2) as D by omega.
       destruct D as [D | [D | [D | [D | D]]]];
         [ (rewrite D in C; simpl in C; discriminate) .. | ].
       pose proof (loadDouble_spec              m       (sub a2 four)) as Sp1.
@@ -338,31 +399,12 @@ Section MemoryHelpers.
       unfold valid_addr in *.
       destruct H, H0.
       rewrite storeDouble_preserves_memSize in Sp2.
-      replace (regToNat  (sub a2 four)) with (regToNat a2 - 4) in *.
-      + assert ((regToNat a2 - 4) mod 8 = 0) as X. {
-          clear Sp1 Sp2.
-          apply Nat.mod_divide; try congruence.
-          change 8 with (2 * 4).
-          assert (((regToNat a2 - 4) / 4) mod 2 = 0) as F. {
-            apply Nat.mod_divides in H4; [ | congruence].
-            destruct H4 as [k Y]. rewrite Y in C|-*.
-            destruct k; [omega|].
-            replace (4 * S k - 4) with (4 * k) by omega.
-            rewrite mul_div_undo in * by congruence.
-            apply Smod2_1. assumption.
-          }
-          replace (regToNat a2 - 4) with ((regToNat a2 - 4) / 4 * 4).
-          - apply Nat.mul_divide_mono_r.
-            apply Nat.mod_divide; congruence.
-          - apply div_mul_undo; try congruence.
-            clear -H4 D. demod. rename H into Y. rewrite Y.
-            rewrite Nat.mod_eq in * by congruence.
-            destruct x; [omega|].
-            replace (4 * S x - 4) with (4 * x) by omega.
-            rewrite mul_div_undo in * by congruence.
-            omega.
+      replace (regToZ_unsigned  (sub a2 four)) with (regToZ_unsigned a2 - 4) in *.
+      + assert ((regToZ_unsigned a2 - 4) mod 8 = 0) as X. {
+          clear Sp1 Sp2 P.
+          div_mod_to_quot_rem. nia.
         }
-        assert (regToNat a2 - 4 + 8 <= memSize m) as A by omega.
+        assert (regToZ_unsigned a2 - 4 + 8 <= memSize m) as A by omega.
         specialize (P (conj A X)).
         rewrite Sp1 in P by (split; assumption). clear Sp1.
         rewrite Sp2 in P by (split; assumption). clear Sp2.
@@ -373,20 +415,20 @@ Section MemoryHelpers.
         }
         specialize (P Ne).
         pose proof combine_inj as Q.
-        specialize (Q 32 32 _ _ _ _ P).
+        specialize (Q 32%nat 32%nat _ _ _ _ P).
         destruct Q as [_ Q].
         ring_simplify (add (sub a2 four) four) in Q.
         assumption.
-      + Check natToReg_semimorph.  rewrite wminus_minus.
-        * rewrite wordToNat_natToWord_idempotent'; [reflexivity|omega].
-        * apply wordToNat_le2.
-          rewrite wordToNat_natToWord_idempotent'; omega.
+      + rewrite sub_def_unsigned.
+        rewrite regToZ_unsigned_four.
+        rewrite regToZ_ZToReg_unsigned; omega.
   Qed.
 
   Lemma loadWord_storeDouble_ne': forall (m : Mem) (a1 a2 : t) (v : word 64),
       in_range a1 8 0 (memSize m) ->
       in_range a2 4 0 (memSize m) ->
-      not_in_range a2 4 regToNat a1 8 -> (* a2 (4 bytes big) is not in the 8-byte range starting at a1 *)
+      (* a2 (4 bytes big) is not in the 8-byte range starting at a1 *)
+      not_in_range a2 4 (regToZ_unsigned a1) 8 ->
       loadWord (storeDouble m a1 v) a2 = loadWord m a2.
   Proof.
     intros.
@@ -395,93 +437,116 @@ Section MemoryHelpers.
     unfold in_range, not_in_range, valid_addr in *;
     simpl in *;
     intuition (subst; try omega);
-    rewrite (wordToNat_wplus' a1 $4) in H6;
-    rewrite wordToNat_natToWord_idempotent' in *;
-    try omega. 
+    rewrite @add_def_unsigned in *;
+    rewrite @regToZ_unsigned_four in *;
+    rewrite @regToZ_ZToReg_unsigned in * by omega;
+    omega.
   Qed.
 
-  Fixpoint store_byte_list(l: list (word 8))(a: t)(m: Mem): Mem :=
-    match l with
-    | nil => m
-    | cons w l' => let m' := storeByte m a w in store_byte_list l' (a ^+ $1) m'
-    end.
+  Definition store_byte_list(l: list (word 8))(a: t)(m: Mem): Mem :=
+    fold_left_index (fun i m w => storeByte m (add a (ZToReg i)) w) l 0 m.
+  
+  Definition load_byte_list(m: Mem)(start: t)(count: Z): list (word 8) :=
+    map_range (fun i => loadByte m (add start (ZToReg i))) count.
 
-  Fixpoint load_byte_list(m: Mem)(start: t)(count: nat): list (word 8) :=
-    match count with
-    | S c => loadByte m start :: load_byte_list m (start ^+ $1) c
-    | O => nil
-    end.
+  Definition store_half_list(l: list (word 16))(a: t)(m: Mem): Mem :=
+    fold_left_index (fun i m w => storeHalf m (add a (ZToReg (2 * i))) w) l 0 m.
 
-  Fixpoint store_half_list(l: list (word 16))(a: t)(m: Mem): Mem :=
-    match l with
-    | nil => m
-    | cons w l' => let m' := storeHalf m a w in store_half_list l' (a ^+ $2) m'
-    end.
+  Definition load_half_list(m: Mem)(start: t)(count: Z): list (word 16) :=
+    map_range (fun i => loadHalf m (add start (ZToReg (2 * i)))) count.
 
-  Fixpoint load_half_list(m: Mem)(start: t)(count: nat): list (word 16) :=
-    match count with
-    | S c => loadHalf m start :: load_half_list m (start ^+ $2) c
-    | O => nil
-    end.
+  Definition store_word_list(l: list (word 32))(a: t)(m: Mem): Mem :=
+    fold_left_index (fun i m w => storeWord m (add a (ZToReg (4 * i))) w) l 0 m.
 
-  Fixpoint store_word_list(l: list (word 32))(a: t)(m: Mem): Mem :=
-    match l with
-    | nil => m
-    | cons w l' => let m' := storeWord m a w in store_word_list l' (a ^+ $4) m'
-    end.
+  Definition load_word_list(m: Mem)(start: t)(count: Z): list (word 32) :=
+    map_range (fun i => loadWord m (add start (ZToReg (4 * i)))) count.
 
-  Fixpoint load_word_list(m: Mem)(start: t)(count: nat): list (word 32) :=
-    match count with
-    | S c => loadWord m start :: load_word_list m (start ^+ $4) c
-    | O => nil
-    end.
+  Definition store_double_list(l: list (word 64))(a: t)(m: Mem): Mem :=
+    fold_left_index (fun i m w => storeDouble m (add a (ZToReg (4 * i))) w) l 0 m.
 
-  Fixpoint store_double_list(l: list (word 64))(a: t)(m: Mem): Mem :=
-    match l with
-    | nil => m
-    | cons w l' => let m' := storeDouble m a w in store_double_list l' (a ^+ $8) m'
-    end.
+  Definition load_double_list(m: Mem)(start: t)(count: Z): list (word 64) :=
+    map_range (fun i => loadDouble m (add start (ZToReg (8 * i)))) count.
 
-  Fixpoint load_double_list(m: Mem)(start: t)(count: nat): list (word 64) :=
-    match count with
-    | S c => loadDouble m start :: load_double_list m (start ^+ $8) c
-    | O => nil
-    end.
-
-  Local Arguments mult: simpl never.
-
-  Lemma nth_error_load_word_list: forall m (l: nat) i offset,
-      i < l ->
-      nth_error (load_word_list m offset l) i =
-      Some (loadWord m (offset ^+ $ (4 * i))).
+  Lemma Znth_error_load_word_list: forall m l i offset,
+      0 <= i < l ->
+      Znth_error (load_word_list m offset l) i =
+      Some (loadWord m (add offset (ZToReg (4 * i)))).
   Proof.
-    induction l; intros; simpl.
-    - exfalso. omega.
-    - destruct i; simpl.
-      + change (4 * 0) with 0. rewrite wplus_comm. rewrite wplus_unit.
-        reflexivity.
-      + replace (offset ^+ $(4 * S i)) with ((offset ^+ $4) ^+ $(4 * i)).
-        * apply IHl. omega.
-        * rewrite <- wplus_assoc. f_equal. rewrite <- natToWord_plus.
-          f_equal. omega.
+    intros. unfold load_word_list.
+    rewrite Znth_error_map_range by assumption.
+    reflexivity.
   Qed.
 
-  Lemma length_load_word_list: forall m l offset,
-      length (load_word_list m offset l) = l.
+  Lemma Zlength_load_word_list: forall m l offset,
+      0 <= l ->
+      Zlength (load_word_list m offset l) = l.
+  Proof.
+    intros. unfold load_word_list.
+    apply Zlength_map_range.
+    assumption.
+  Qed.
+
+  Local Arguments Z.mul: simpl never.
+
+  Lemma fold_left_index_cons': forall T R (a: T) (l: list T) (f: Z -> R -> T -> R) (i: Z) (r: R),
+      fold_left_index f (a :: l) i r = fold_left_index f l (i + 1) (f i r a).
+  Proof.
+    intros. reflexivity.
+  Qed.
+
+  Lemma fold_left_index_shift: forall T R (l: list T) (f: Z -> R -> T -> R) (i d: Z) (r: R),
+      fold_left_index f l (i + d) r = fold_left_index (fun j => f (j + d)) l i r.
   Proof.
     induction l; intros.
     - reflexivity.
-    - simpl. f_equal. apply IHl.
+    - unfold fold_left_index in *. simpl in *.
+      replace (i + d + 1) with (i + 1 + d) by omega.
+      apply IHl.
   Qed.
 
-  Local Arguments mult: simpl never.
+  Lemma fold_left_index_cons: forall T R (a: T) (l: list T) (f: Z -> R -> T -> R) (i: Z) (r: R),
+      fold_left_index f (a :: l) i r =
+      fold_left_index (fun i => f (i + 1)) l i (f i r a).
+  Proof.
+    intros. rewrite fold_left_index_cons'. apply fold_left_index_shift.
+  Qed.
+
+  Lemma fold_left_ext: forall A B (f1 f2: A -> B -> A) (l: list B) (a0: A),
+      (forall a b, f1 a b = f2 a b) ->
+      fold_left f1 l a0 = fold_left f2 l a0.
+  Proof.
+    induction l; intros.
+    - reflexivity.
+    - simpl. rewrite H. apply IHl. assumption.
+  Qed.
+  
+  Lemma store_word_list_cons: forall w l a m,
+      store_word_list (w :: l) a m = store_word_list l (add a four) (storeWord m a w).
+  Proof.
+    intros. unfold store_word_list. rewrite fold_left_index_cons.
+    rewrite Z.mul_0_r.
+    rewrite ZToReg_morphism.(morph0).
+    ring_simplify (add a zero).
+    unfold fold_left_index.
+    f_equal.
+    apply fold_left_ext.
+    intros. do 2 f_equal.
+    rewrite! add_def_unsigned.
+    rewrite! regToZ_unsigned_four.
+    rewrite! ZToReg_morphism.(morph_mul).
+    rewrite! ZToReg_morphism.(morph_add).
+    rewrite! ZToReg_regToZ_unsigned.
+    rewrite! ZToReg_morphism.(morph1).
+    ring.
+  Qed.
 
   Lemma store_word_list_preserves_memSize_aux: forall ll (m: Mem) a l,
       length l = ll ->
       memSize (store_word_list l a m) = memSize m.
   Proof.
-    induction ll; intros; subst; destruct l; simpl in *; try congruence.
+    induction ll; intros; subst; destruct l; simpl in *; try reflexivity; try congruence.
     inversion H; subst.
+    rewrite store_word_list_cons.
     rewrite IHll by reflexivity.
     apply storeWord_preserves_memSize.
   Qed.
@@ -493,11 +558,19 @@ Section MemoryHelpers.
   Qed.
  
   Lemma loadWord_before_store_word_list: forall l (m: Mem) (a1 a2: t),
-      regToNat a1 + 4 <= regToNat a2 ->
-      regToNat a2 + 4 * (length l) <= (memSize m) ->
+      regToZ_unsigned a1 + 4 <= regToZ_unsigned a2 ->
+      regToZ_unsigned a2 + 4 * (Zlength l) <= (memSize m) ->
       valid_addr a1 4 (memSize m) ->
       valid_addr a2 4 (memSize m) ->
-      loadWord (store_word_list l a2 m) a1  = loadWord m a1.
+      loadWord (store_word_list l a2 m) a1 = loadWord m a1.
+  Proof.
+    induction l; intros; unfold store_word_list in *; simpl in *; try reflexivity.
+    mem_simpl.
+    destruct_list_length; simpl in *.
+    - mem_simpl.
+    - rewrite IHl; mem_simpl.
+  Qed.
+
   Proof.
     induction l; intros; simpl in *; try congruence.
     mem_simpl.
@@ -507,7 +580,7 @@ Section MemoryHelpers.
   Qed.
 
   Lemma loadWord_after_store_word_list: forall l (m: Mem) (a1 a2: t),
-      regToNat a2 + 4 * (length l) <= regToNat a1 ->
+      regToZ_unsigned a2 + 4 * (length l) <= regToZ_unsigned a1 ->
       valid_addr a1 4 (memSize m) ->
       valid_addr a2 4 (memSize m) ->
       loadWord (store_word_list l a2 m) a1 = loadWord m a1.
@@ -520,8 +593,8 @@ Section MemoryHelpers.
   Qed.
 
   Lemma loadWord_outside_store_word_list: forall l (m: Mem) a1 a2,
-      not_in_range a1 4 regToNat a2 (4 * length l) ->
-      regToNat a2 + 4 * length l <= memSize m ->
+      not_in_range a1 4 (regToZ_unsigned a2) (4 * Zlength l) ->
+      regToZ_unsigned a2 + 4 * Zlength l <= memSize m ->
       valid_addr a1 4 (memSize m) ->
       valid_addr a2 4 (memSize m) ->
       loadWord (store_word_list l a2 m) a1 = loadWord m a1.
@@ -542,9 +615,9 @@ Section MemoryHelpers.
 
   Lemma loadWord_inside_store_word_list_aux: forall l (m: Mem) i offset,
       i < length l ->
-      regToNat offset + 4 * length l <= memSize m ->
+      regToZ_unsigned offset + 4 * length l <= memSize m ->
       valid_addr offset 4 (memSize m) ->
-      loadWord (store_word_list l offset m) $(regToNat offset + 4 * i) = nth i l $0.
+      loadWord (store_word_list l offset m) $(regToZ_unsigned offset + 4 * i) = nth i l $0.
   Proof.
     induction l; intros; unfold in_range in *; simpl in *; mem_simpl.
     destruct_list_length; simpl in *.
@@ -557,13 +630,13 @@ Section MemoryHelpers.
   Qed.
   
   Lemma loadWord_inside_store_word_list: forall l (m: Mem) addr offset,
-      in_range addr 4 regToNat offset (4 * length l) ->
-      regToNat offset + 4 * length l <= memSize m ->
+      in_range addr 4 regToZ_unsigned offset (4 * length l) ->
+      regToZ_unsigned offset + 4 * length l <= memSize m ->
       valid_addr offset 4 (memSize m) ->
-      loadWord (store_word_list l offset m) addr = nth (regToNat  (addr ^- offset) / 4) l $0.
+      loadWord (store_word_list l offset m) addr = nth (regToZ_unsigned  (addr ^- offset) / 4) l $0.
   Proof.
     intros. unfold in_range in *.
-    rewrite <- (loadWord_inside_store_word_list_aux l m (regToNat  (addr ^- offset) / 4) offset);
+    rewrite <- (loadWord_inside_store_word_list_aux l m (regToZ_unsigned  (addr ^- offset) / 4) offset);
       try assumption.
     (* TODO this should be in mem_simpl too *)
     - repeat f_equal. rewrite wminus_minus' by omega.
@@ -577,8 +650,8 @@ Section MemoryHelpers.
   Qed.
   
   Lemma loadDouble_before_store_word_list: forall l (m: Mem) (a1 a2: t),
-      regToNat a1 + 8 <= regToNat a2 ->
-      regToNat a2 + 4 * (length l) <= (memSize m) ->
+      regToZ_unsigned a1 + 8 <= regToZ_unsigned a2 ->
+      regToZ_unsigned a2 + 4 * (length l) <= (memSize m) ->
       valid_addr a1 8 (memSize m) ->
       valid_addr a2 4 (memSize m) ->
       loadDouble (store_word_list l a2 m) a1  = loadDouble m a1.
@@ -591,7 +664,7 @@ Section MemoryHelpers.
   Qed.
 
   Lemma loadDouble_after_store_word_list: forall l (m: Mem) (a1 a2: t),
-      regToNat a2 + 4 * (length l) <= regToNat a1 ->
+      regToZ_unsigned a2 + 4 * (length l) <= regToZ_unsigned a1 ->
       valid_addr a1 8 (memSize m) ->
       valid_addr a2 4 (memSize m) ->
       loadDouble (store_word_list l a2 m) a1  = loadDouble m a1.
@@ -604,8 +677,8 @@ Section MemoryHelpers.
   Qed.
 
   Lemma loadDouble_outside_store_word_list: forall l (m: Mem) a1 a2,
-      not_in_range a1 8 regToNat a2 (4 * length l) ->
-      regToNat a2 + 4 * length l <= memSize m ->
+      not_in_range a1 8 regToZ_unsigned a2 (4 * length l) ->
+      regToZ_unsigned a2 + 4 * length l <= memSize m ->
       valid_addr a1 8 (memSize m) ->
       valid_addr a2 4 (memSize m) ->
       loadDouble (store_word_list l a2 m) a1 = loadDouble m a1.
@@ -620,8 +693,8 @@ Section MemoryHelpers.
   Lemma load_store_word_list_eq: forall l (m: Mem) ll a1 a2,
       a2 = a1 ->
       ll = length l ->
-      regToNat a1 mod 4 = 0 ->
-      regToNat a1 + 4 * (length l) <= memSize m ->
+      regToZ_unsigned a1 mod 4 = 0 ->
+      regToZ_unsigned a1 + 4 * (length l) <= memSize m ->
       load_word_list (store_word_list l a1 m) a2 ll = l.
   Proof.
     induction l; intros; subst; simpl in *; try congruence.
